An application of the Z property

src/ZtoConfl.v
@@ -2,6 +2,14 @@ Definition Rel (A:Type) := A -> A -> Prop.
 
 Definition NF {A:Type} (a:A) (R: Rel A) := ~(exists b, R a b).
 
+(* Transitive closure of a reduction relation *)
+Inductive trans {A} (red: Rel A) : Rel A :=
+| singl: forall a b,  red a b -> trans red a b
+| transit: forall b a c,  red a b -> trans red b c -> trans red a c
+.
+
+Arguments transit {A} {red} _ _ _ _ _ .
+
 Inductive refltrans {A:Type} (R: Rel A) : A -> A -> Prop :=
 | refl: forall a, (refltrans R) a a
 | rtrans: forall a b c, R a b -> refltrans R b c -> refltrans R a c.
@@ -97,3 +105,202 @@ Proof.
            assumption.
 Qed.
 
+(** Confluence of the Lex-calculus *)
+
+Definition var := nat.
+
+Require Import Arith MSetList.
+
+Declare Module Var_as_OT : UsualOrderedType
+  with Definition t := var.
+Module Import VarSet := MSetList.Make Var_as_OT.
+
+Definition vars := VarSet.t.
+
+Notation "{}" := (VarSet.empty).
+Notation "{{ x }}" := (VarSet.singleton x).
+Notation "s [=] t " := (VarSet.Equal s t) (at level 70, no associativity). 
+Notation "E \u F" := (VarSet.union E F)  (at level 68, left associativity).
+Notation "x \in E" := (VarSet.In x E) (at level 69).
+Notation "x \notin E" := (~ VarSet.In x E) (at level 69).
+Notation "E << F" := (VarSet.Subset E F) (at level 70, no associativity).
+Notation "E \rem F" := (VarSet.remove F E) (at level 70).
+
+Lemma eq_var_dec : forall x y : var, {x = y} + {x <> y}.
+Proof. exact eq_nat_dec. Qed.
+
+Notation "x == y" := (eq_var_dec x y) (at level 67).
+Notation "i === j" := (Peano_dec.eq_nat_dec i j) (at level 67).
+
+Inductive pterm : Set :=
+  | pterm_bvar : nat -> pterm
+  | pterm_fvar : var -> pterm
+  | pterm_app  : pterm -> pterm -> pterm
+  | pterm_abs  : pterm -> pterm
+  | pterm_sub : pterm -> pterm -> pterm.
+
+Notation "t [ u ]" := (pterm_sub t u) (at level 70).
+
+(** Opening up abstractions and substitutions *)
+Fixpoint open_rec (k : nat) (u : pterm) (t : pterm) {struct t} : pterm :=
+  match t with
+  | pterm_bvar i    => if k === i then u else (pterm_bvar i)
+  | pterm_fvar x    => pterm_fvar x
+  | pterm_app t1 t2 => pterm_app (open_rec k u t1) (open_rec k u t2)
+  | pterm_abs t1    => pterm_abs (open_rec (S k) u t1)
+  | pterm_sub t1 t2 => pterm_sub (open_rec (S k) u t1) (open_rec k u t2)
+  end.
+
+Definition open t u := open_rec 0 u t.
+
+Notation "{ k ~> u } t" := (open_rec k u t) (at level 67).
+Notation "t ^^ u" := (open t u) (at level 67). 
+Notation "t ^ x" := (open t (pterm_fvar x)).   
+
+(** Variable closing *)
+Fixpoint close_rec  (k : nat) (x : var) (t : pterm) {struct t} : pterm :=
+  match t with
+  | pterm_bvar i    => pterm_bvar i
+  | pterm_fvar x'    => if x' == x then (pterm_bvar k) else pterm_fvar x'
+  | pterm_app t1 t2 => pterm_app (close_rec k x t1) (close_rec k x t2)
+  | pterm_abs t1    => pterm_abs (close_rec (S k) x t1)
+  | pterm_sub t1 t2 => pterm_sub (close_rec (S k) x t1) (close_rec k x t2)
+  end.
+
+Definition close t x := close_rec 0 x t.
+
+(** ES terms are expressions without dangling deBruijn indexes. *)
+Inductive term : pterm -> Prop :=
+  | term_var : forall x,
+      term (pterm_fvar x)
+  | term_app : forall t1 t2,
+      term t1 -> 
+      term t2 -> 
+      term (pterm_app t1 t2)
+  | term_abs : forall L t1,
+      (forall x, x \notin L -> term (t1 ^ x)) ->
+      term (pterm_abs t1)
+  | term_sub : forall L t1 t2,
+     (forall x, x \notin L -> term (t1 ^ x)) ->
+      term t2 -> 
+      term (pterm_sub t1 t2).
+Hint Constructors term.
+
+(** Local closure of terms *)
+Fixpoint lc_at (k:nat) (t:pterm) : Prop :=
+  match t with
+  | pterm_bvar i    => i < k
+  | pterm_fvar x    => True
+  | pterm_app t1 t2 => lc_at k t1 /\ lc_at k t2
+  | pterm_abs t1    => lc_at (S k) t1
+  | pterm_sub t1 t2 => (lc_at (S k) t1) /\ lc_at k t2
+  end.
+
+Definition body t := exists L, forall x, x \notin L -> term (t ^ x).
+
+Fixpoint bswap_rec (k : nat) (t : pterm) : pterm :=
+  match t with
+  | pterm_bvar i    => if k === i then (pterm_bvar (S k))
+                       else (if (S k) === i then (pterm_bvar k) else t)
+  | pterm_fvar x    => t
+  | pterm_app t1 t2 => pterm_app (bswap_rec k t1) (bswap_rec k t2)
+  | pterm_abs t1    => pterm_abs (bswap_rec (S k) t1)
+  | pterm_sub t1 t2 => pterm_sub (bswap_rec (S k) t1) (bswap_rec k t2)
+  end.
+
+Definition bswap t := bswap_rec 0 t.
+Notation "& t" := (bswap t) (at level 67).
+
+(** bswap replaces 0s by 1s and vice-versa. Any other index is preserved. *)
+Fixpoint has_free_index (k:nat) (t:pterm) : Prop :=
+  match t with
+    | pterm_bvar n => if (k === n) then True else False
+    | pterm_fvar x => False
+    | pterm_app t1 t2 => (has_free_index k t1) \/ (has_free_index k t2)
+    | pterm_abs t1 => has_free_index (S k) t1
+    | pterm_sub t1 t2 => (has_free_index (S k) t1) \/ (has_free_index k t2)
+  end.
+
+Lemma has_index: forall i, has_free_index i (pterm_bvar i).
+Proof.
+  intro i. simpl. case (i === i).
+  - intro. auto.
+  - intro. apply n. reflexivity.
+Qed.  
+
+Lemma bswap_preserves: forall t, ~(has_free_index 0 t) -> ~(has_free_index 1 t) -> & t = t.
+Proof.
+  intro t. unfold bswap. generalize 0.
+  generalize dependent t. induction t0.
+  - intros n' Hn HSn. unfold bswap_rec.
+    destruct (n' === n) as [ Heq | Hdiff ]; subst.
+    + apply False_ind. apply Hn. apply has_index.
+    + destruct (S n' === n) as [ HSeq | HSdiff ]; subst.
+      * apply False_ind. apply HSn. apply has_index.        
+      * reflexivity.
+  - intros n Hn HSn. reflexivity.
+  - intros n Hn HSn. simpl in *. apply Decidable.not_or in Hn.
+    destruct Hn as [ Hnt1 Hnt2 ]. apply Decidable.not_or in HSn.
+    destruct HSn as [ HSnt1 HSnt2 ]. rewrite IHt0_1. rewrite IHt0_2. reflexivity.
+    assumption. assumption. assumption. assumption.          
+  - intros n Hn HSn. simpl in *. rewrite IHt0. reflexivity. 
+    intro HSn'. apply Hn. assumption. intro HSSn. apply HSn. assumption.
+  - intros n Hn HSn. simpl in *. apply Decidable.not_or in Hn.
+    destruct Hn as [ Hnt1 Hnt2 ]. apply Decidable.not_or in HSn.
+    destruct HSn as [ HSnt1 HSnt2 ]. rewrite IHt0_1. rewrite IHt0_2. reflexivity.
+    assumption. assumption. assumption. assumption.
+Qed.  
+
+(** Contextual closure of terms. *)
+Inductive ES_contextual_closure (R: Rel pterm) : Rel pterm :=
+  | ES_redex : forall t s, R t s -> ES_contextual_closure R t s
+  | ES_app_left : forall t t' u, term u -> ES_contextual_closure R t t' ->
+	  		      ES_contextual_closure R (pterm_app t u) (pterm_app t' u)
+  | ES_app_right : forall t u u', term t -> ES_contextual_closure R u u' ->
+	  		       ES_contextual_closure R (pterm_app t u) (pterm_app t u')
+  | ES_abs_in : forall t t' L, (forall x, x \notin L -> ES_contextual_closure R (t^x) (t'^x)) ->
+                               ES_contextual_closure R (pterm_abs t) (pterm_abs t')
+  | ES_subst_left : forall t t' u L, term u ->
+                                     (forall x, x \notin L -> ES_contextual_closure R (t^x) (t'^x)) ->
+	                             ES_contextual_closure R  (t [u]) (t' [u])
+  | ES_subst_right : forall t u u', body t -> ES_contextual_closure R u u' ->
+	  	                    ES_contextual_closure R  (t [u]) (t [u']).
+
+Inductive eqc : Rel pterm :=
+| eqc_def: forall t u v, lc_at 2 t -> term u -> term v -> eqc (t[u][v]) ((& t)[v][u]).
+Definition eqc_ctx (t u: pterm) := ES_contextual_closure eqc t u.
+Notation "t =c u" := (eqc_ctx t u) (at level 66).
+Definition eqc_trans (t u: pterm) := trans eqc_ctx t u.
+Notation "t =c+ u" := (eqc_trans t u) (at level 66).
+Definition eqC (t : pterm) (u : pterm) := refltrans eqc_ctx t u.
+Notation "t =e u" := (eqC t u) (at level 66).
+
+Definition red_ctx_mod_eqC (R: Rel pterm) (t: pterm) (u : pterm) :=
+           exists t', exists u', (t =e t')/\(R t' u')/\(u' =e u).
+
+Inductive rule_b : pterm -> pterm -> Prop :=
+   reg_rule_b : forall (t u:pterm),  body t -> term u ->  
+     rule_b (pterm_app(pterm_abs t) u) (t[u]).
+Notation "t ->_B u" := (rule_b t u) (at level 66).
+
+Inductive sys_x : Rel pterm :=
+| reg_rule_var : forall t, sys_x (pterm_bvar 0 [t]) t
+| reg_rule_gc : forall t u, term t -> sys_x (t[u]) t
+| reg_rule_app : forall t1 t2 u, 
+  sys_x ((pterm_app t1 t2)[u]) (pterm_app (t1[u]) (t2[u]))
+| reg_rule_lamb : forall t u, 
+  sys_x ((pterm_abs t)[u]) (pterm_abs ((& t)[u]))
+| reg_rule_comp : forall t u v, has_free_index 0 u ->
+  sys_x (t[u][v]) (((& t)[v])[ u[ v ] ]).
+
+Notation "t ->_x u" := (sys_x t u) (at level 59, left associativity).
+
+Inductive sys_Bx: Rel pterm :=
+| B_lx : forall t u, t ->_B u -> sys_Bx t u
+| sys_x_lx : forall t u, t ->_x u -> sys_Bx t u.
+
+Definition lex t u :=  red_ctx_mod_eqC sys_Bx t u.
+
+Theorem Zlex: Zprop lex.
+Proof.
+Admitted.
